HOL/DataStrs/Reverse_Func.thy
@@ -2,52 +2,7 @@ theory Reverse_Func
 imports "../Auto2_Main"
 begin
 
-section {* Results about nth *}
-
-setup {* register_wellform_data ("xs ! i", ["i < length xs"]) *}
-setup {* add_rewrite_rule @{thm List.nth_append} *}
-setup {* add_rewrite_rule @{thm List.nth_Cons'} *}
-
-section {* Basic definitions *}
-
-setup {* fold add_rewrite_rule @{thms List.rev.simps} *}
-
-lemma rev_one [rewrite]: "rev [x] = [x]" by simp
-
-lemma rev_append [rewrite]: "rev (xs @ ys) = rev ys @ rev xs"
-@proof @induct xs @qed
-
-lemma rev_length: "length (rev xs) = length xs"
-@proof @induct xs @qed
-setup {* add_forward_prfstep_cond @{thm rev_length} [with_term "rev ?xs"] *}
-
-lemma nat_sub1 [rewrite]: "(a::nat) - n - 1 = a - 1 - n" by simp
-
-lemma rev_nth [rewrite]:
-  "n < length xs \<Longrightarrow> rev xs ! n = xs ! (length xs - 1 - n)"
-@proof @induct xs @qed
-
-section {* Linear time version of rev *}
-
-fun itrev :: "'a list \<Rightarrow> 'a list \<Rightarrow> 'a list" where
-  "itrev []       ys = ys" |
-  "itrev (x # xs) ys = itrev xs (x # ys)"
-setup {* fold add_rewrite_rule @{thms itrev.simps} *}
-
-lemma itrev_eq_rev: "itrev x [] = rev x"
-@proof
-  @have (@rule) "\<forall>y. itrev x y = rev x @ y" @with
-    @induct x arbitrary y @with
-      @subgoal "x = a # b" @have "a # y = [a] @ y" @endgoal
-    @end
-  @end
-@qed
-
-section {* List update *}
-
-setup {* register_wellform_data ("xs[i := x]", ["i < length xs"]) *}
-setup {* add_rewrite_rule @{thm List.nth_list_update} *}
-setup {* add_forward_prfstep_cond @{thm List.length_list_update} [with_term "?xs[?i := ?x]"] *}
+section {* List swap *}
 
 definition list_swap :: "'a list \<Rightarrow> nat \<Rightarrow> nat \<Rightarrow> 'a list" where
   "list_swap xs i j = xs[i := xs ! j, j := xs ! i]"
@@ -61,8 +16,8 @@ lemma list_swap_eval:
 setup {* add_rewrite_rule_cond @{thm list_swap_eval} [with_cond "?k \<noteq> ?i", with_cond "?k \<noteq> ?j"] *}
 
 lemma list_swap_eval_triv [rewrite]:
-  "i < length xs \<Longrightarrow> (list_swap xs i j) ! i = xs ! j"
-  "j < length xs \<Longrightarrow> (list_swap xs i j) ! j = xs ! i" by auto2+
+  "i < length xs \<Longrightarrow> j < length xs \<Longrightarrow> (list_swap xs i j) ! i = xs ! j"
+  "i < length xs \<Longrightarrow> j < length xs \<Longrightarrow> (list_swap xs i j) ! j = xs ! i" by auto2+
 
 lemma length_list_swap:
   "length (list_swap xs i j) = length xs" by auto2
@@ -73,7 +28,13 @@ lemma mset_list_swap [rewrite]:
 setup {* del_prfstep_thm @{thm list_swap_def} *}
 setup {* add_rewrite_rule_back @{thm list_swap_def} *}
 
-section {* Definition of rev in terms of swaps *}
+section {* Reverse *}
+
+lemma nat_sub1 [rewrite]: "(a::nat) - n - 1 = a - 1 - n" by simp
+
+lemma rev_nth [rewrite]:
+  "n < length xs \<Longrightarrow> rev xs ! n = xs ! (length xs - 1 - n)"
+@proof @induct xs @qed
   
 fun rev_swap :: "'a list \<Rightarrow> nat \<Rightarrow> nat \<Rightarrow> 'a list" where
   "rev_swap xs i j = (if i < j then rev_swap (list_swap xs i j) (i + 1) (j - 1) else xs)"
@@ -96,7 +57,8 @@ lemma nat_sub2 [rewrite]: "(k::nat) \<ge> i + 1 \<Longrightarrow> j - 1 - (k - (
 lemma rev_swap_eval [rewrite]:
   "j < length xs \<Longrightarrow> (rev_swap xs i j) ! k =
     (if k < i then xs ! k else if k > j then xs ! k else xs ! (j - (k - i)))"
-@proof @strong_induct j arbitrary i xs
+@proof
+  @strong_induct j arbitrary i xs
   @case "i < j" @with
     @let "xs' = list_swap xs i j"
     @apply_induct_hyp "j - 1" "i + 1" xs'
@@ -107,27 +69,6 @@ lemma rev_swap_eval [rewrite]:
 
 lemma rev_swap_is_rev [rewrite]:
   "length xs \<ge> 1 \<Longrightarrow> rev_swap xs 0 (length xs - 1) = rev xs" by auto2
-
-section {* take *}
-
-setup {* register_wellform_data ("take n xs", ["n \<le> length xs"]) *}
-setup {* add_prfstep_check_req ("take n xs", "n \<le> length xs") *}
-
-lemma length_take: "n \<le> length xs \<Longrightarrow> length (take n xs) = n" by simp
-setup {* add_rewrite_rule_cond @{thm length_take} [with_term "take ?n ?xs"] *}
-
-lemma nth_take [rewrite]: "i < length (take n xs) \<Longrightarrow> take n xs ! i = xs ! i" by simp
-
-setup {* add_rewrite_rule @{thm List.take_0} *}
-
-section {* drop *}
-
-setup {* add_rewrite_rule_cond @{thm List.length_drop} [with_term "drop ?n ?xs"] *}
-
-lemma nth_drop [rewrite]: "i < length (drop n xs) \<Longrightarrow> drop n xs ! i = xs ! (n + i)" by simp
-
-setup {* add_rewrite_rule @{thm List.drop_0} *}
-setup {* add_rewrite_rule @{thm List.drop_all} *}
 
 section {* Copy one array to the beginning of another *}
     
@@ -150,12 +91,13 @@ setup {* add_forward_prfstep_cond @{thm array_copy_length} [with_term "array_cop
 lemma nat_sub6 [rewrite]: "(a::nat) + (b + 1) - (c + 1) = a + b - c" by simp
 
 lemma array_copy_eval [rewrite]:
-  "i + n \<le> length xs \<Longrightarrow> j + n \<le> length xs' \<Longrightarrow> (array_copy xs i xs' j n) ! k =
-   (if k < j then xs' ! k else if k \<ge> j + n then xs' ! k else xs ! (k + i - j))"
+  "i + n \<le> length xs \<Longrightarrow> j + n \<le> length xs' \<Longrightarrow>
+   (array_copy xs i xs' j n) ! k = (if k < j then xs' ! k else if k \<ge> j + n then xs' ! k else xs ! (k + i - j))"
 @proof
   @strong_induct n arbitrary i j xs'
   @case "n = 0" @then
   @apply_induct_hyp "n - 1" "i + 1" "j + 1" "xs' [j := xs ! i]"
+  @case "k < j" @then @case "k \<ge> j + n" @then @have "k < length xs'"
 @qed
 
 setup {* del_prfstep_thm @{thm array_copy.simps} *}
@@ -192,7 +134,7 @@ lemma sublist_single [rewrite]:
 lemma nat_sub7 [rewrite]: "b \<le> a \<Longrightarrow> c \<le> b \<Longrightarrow> ((a::nat) - b) + (b - c) = a - c" by simp
 lemma nat_sub8 [rewrite]: "b \<ge> c \<Longrightarrow> a \<ge> b - c \<Longrightarrow> (a::nat) - (b - c) + b = a + c" by simp
 
-lemma sublist_as_append [rewrite]:
+lemma sublist_append [rewrite]:
   "l \<le> m \<Longrightarrow> m \<le> r \<Longrightarrow> r \<le> length xs \<Longrightarrow> sublist l m xs @ sublist m r xs = sublist l r xs"
 @proof
   @let "xs1 = sublist l r xs" "xs2 = sublist l m xs" "xs3 = sublist m r xs"
@@ -203,28 +145,27 @@ lemma sublist_as_append [rewrite]:
   @end
 @qed
 
-lemma sublist_as_Cons [rewrite]:
+lemma sublist_Cons [rewrite]:
   "r \<le> length xs \<Longrightarrow> l < r \<Longrightarrow> xs ! l # sublist (l + 1) r xs = sublist l r xs"
 @proof
   @have "sublist l r xs = sublist l (l + 1) xs @ sublist (l + 1) r xs"
 @qed
 
-lemma sorted_triv_list [backward]:
+lemma sorted_triv_sublist [backward]:
   "r + 1 \<le> length xs \<Longrightarrow> l \<ge> r \<Longrightarrow> sorted (sublist l (r + 1) xs)"
 @proof @case "l = r" @qed
 
-setup {* add_rewrite_rule @{thm sorted_append} *}
 lemma sorted_pivoted_list [forward]:
   "l \<le> p \<Longrightarrow> p + 1 \<le> r \<Longrightarrow> r \<le> length xs \<Longrightarrow>
    sorted (sublist (p + 1) r xs) \<Longrightarrow> sorted (sublist l p xs) \<Longrightarrow>
    \<forall>x\<in>set (sublist l p xs). x \<le> xs ! p \<Longrightarrow> \<forall>y\<in>set (sublist (p + 1) r xs). xs ! p \<le> y \<Longrightarrow>
    sorted (sublist l r xs)"
 @proof
-  @have "sublist p r xs = (xs ! p) # sublist (p + 1) r xs" @then
+  @have "sublist p r xs = (xs ! p) # sublist (p + 1) r xs"
+  @have "sorted (sublist p r xs)"
   @case "p = 0"
   @have "sublist l r xs = sublist l p xs @ sublist p r xs"
 @qed
-setup {* del_prfstep_thm @{thm sorted_append} *}
 
 lemma sublist_equalityI:
   "i \<le> j \<Longrightarrow> j \<le> length xs \<Longrightarrow> length xs = length ys \<Longrightarrow>
@@ -239,7 +180,7 @@ lemma set_sublist [resolve]:
   "j \<le> length xs \<Longrightarrow> x \<in> set (sublist i j xs) \<Longrightarrow> \<exists>k. k \<ge> i \<and> k < j \<and> x = xs ! k"
 @proof
   @let "xs' = sublist i j xs" @have "length xs' = j - i"
-  @obtain l where "l < length xs'" "x = xs' ! l"
+  @obtain l where "l < length xs'" "xs' ! l = x"
   @have "x = xs ! (l + i)"
   @have "i + l \<ge> i"
 @qed
@@ -250,9 +191,5 @@ lemma list_take_sublist_drop_eq [rewrite]:
   @have "take l xs = sublist 0 l xs" @with @have "length (take l xs) = l" @end
   @have "drop r xs = sublist r (length xs) xs" @with @have "length (drop r xs) = length xs - r" @end
 @qed
-
-setup {* add_rewrite_rule @{thm mset_append} *}
-setup {* add_forward_prfstep @{thm add_right_imp_eq} *}
-setup {* add_forward_prfstep @{thm add_left_imp_eq} *}
 
 end
