HOL/Lists_Thms.thy
@@ -1,110 +1,147 @@
 (* Setup for proof steps related to lists. *)
 
 theory Lists_Thms
-imports Auto2_HOL
+imports Set_Thms
 begin
 
-section {* Case checking and induction *}
+section {* Definition of lists *}
 
 setup {* add_resolve_prfstep @{thm list.distinct(2)} *}
-theorem list_constr [forward]: "x # xs = y # ys \<Longrightarrow> x = y \<and> xs = ys" by simp
+setup {* add_forward_prfstep (equiv_forward_th @{thm list.simps(1)}) *}
 setup {* fold add_rewrite_rule @{thms List.list.sel(1,3)} *}
-setup {* add_rewrite_rule @{thm List.hd_append2} *}
 setup {* add_forward_prfstep @{thm list.collapse} *}
-
-text {* Induction. After proving a property P holds for [], can assume P holds
-  for tl l when trying to show P l. *}
-
 setup {* add_var_induct_rule @{thm list.induct} *}
 
-section {* Other functions *}
+section {* Append *}
 
-subsection {* append *}
-
-theorem list_append_one [rewrite]: "[a] @ b = a # b" by simp
-setup {* add_rewrite_rule_cond @{thm List.append.simps(2)} [with_cond "?xs \<noteq> []"] *}
-theorem append_eq_empty [forward]: "xs @ ys = [] \<Longrightarrow> xs = [] \<and> ys = []" by simp
+setup {* add_rewrite_rule @{thm List.append.simps(2)} *}
+setup {* add_rewrite_rule @{thm List.hd_append2} *}
 
 setup {* ACUtil.add_ac_data {
   cfhead = @{cterm "op @"}, assoc_th = @{thm List.append_assoc}, comm_th = true_th,
   unitl_th = @{thm List.append.append_Nil}, unitr_th = @{thm List.append_Nil2}}
 *}
 
-subsection {* length *}
+lemma append_is_empty [forward]: "xs @ ys = [] \<Longrightarrow> xs = [] \<and> ys = []" by simp
 
-theorem length_Cons [rewrite]: "length (a # b) = length b + 1" by simp
-setup {* add_rewrite_rule @{thm length_replicate} *}
+section {* length *}
+
 setup {* add_rewrite_rule @{thm List.list.size(3)} *}
-setup {* add_rewrite_rule @{thm List.length_append} *}
 theorem length_one [rewrite]: "length [x] = 1" by simp
-theorem length_tl' [rewrite]: "l' \<noteq> [] \<Longrightarrow> length (tl l') + 1 = length l'" by simp
-setup {* add_rewrite_rule_back_cond @{thm List.length_list_update} [with_term "list_update ?xs ?i ?x"] *}
-setup {* add_rewrite_rule @{thm length_butlast} *}
-theorem length_butlast': "xs \<noteq> [] \<Longrightarrow> length xs = length (butlast xs) + 1" by simp
-setup {* add_forward_prfstep_cond @{thm length_butlast'} [with_term "length (butlast ?xs)"] *}
-
-theorem list_last_singleton [rewrite]: "length xs = 1 \<Longrightarrow> last xs = hd xs"
-  by (metis diff_is_0_eq hd_conv_nth last_conv_nth le_numeral_extra(4) length_greater_0_conv zero_less_one)
-
-subsection {* nth *}
-
-theorem nth_append1 [rewrite]: "i < length xs \<Longrightarrow> (xs @ ys) ! i = xs ! i" by (simp add: nth_append)
-setup {* add_rewrite_rule_back @{thm hd_conv_nth} *}
-setup {* add_rewrite_rule @{thm nth_butlast} *}
-setup {* add_rewrite_rule @{thm List.nth_list_update_neq} *}
-setup {* add_rewrite_rule @{thm List.nth_list_update_eq} *}
-setup {* add_rewrite_rule @{thm List.nth_append_length} *}
-setup {* add_rewrite_rule @{thm List.nth_replicate} *}
-
-subsection {* sorted *}
-
-setup {* add_property_const @{term sorted} *}
-setup {* fold add_resolve_prfstep [@{thm sorted.Nil}, @{thm sorted_single}] *}
-  
-lemma sorted_ConsI [backward]: "sorted xs \<and> (\<forall>y\<in>set xs. x \<le> y) \<Longrightarrow> sorted (x # xs)"
-  by (simp add: sorted_Cons)
-
-lemma sorted_ConsD1 [forward]: "sorted (x # xs) \<Longrightarrow> sorted xs" using sorted_Cons by blast
-lemma sorted_ConsD2 [forward, backward2]: "sorted (x # xs) \<Longrightarrow> y \<in> set xs \<Longrightarrow> x \<le> y"
-  using sorted_Cons by blast  
-
-lemma sorted_appendI [forward]:
-  "sorted xs \<Longrightarrow> sorted ys \<Longrightarrow> \<forall>x\<in>set xs. \<forall>y\<in>set ys. x \<le> y \<Longrightarrow> sorted (xs @ ys)"
-  by (simp add: sorted_append)
-
-subsection {* distinct *}
-
-theorem distinct2 [rewrite]: "distinct [a, b] = (a \<noteq> b)" by simp
-theorem distinct3 [rewrite]: "distinct [a, b, c] = (a \<noteq> b \<and> a \<noteq> c \<and> b \<noteq> c)" by simp
-setup {* add_rewrite_rule @{thm distinct.simps(1)} #>
-  add_resolve_prfstep @{thm distinct_singleton} #>
-  add_rewrite_rule_cond @{thm distinct.simps(2)} (
-    with_conds ["?xs \<noteq> []", "?xs \<noteq> [?a]", "?xs \<noteq> [?a, ?b]"]) *}
-
-section {* Set of elements of a list *}
-
-setup {* add_rewrite_rule @{thm List.set_simps(1)} *}
-theorem set_list_single [rewrite]: "set [x] = {x}" by simp
-theorem set_list_simp2: "set (x # xs) = {x} \<union> set xs" by simp
-setup {* add_rewrite_rule_cond @{thm set_list_simp2} [with_cond "?xs \<noteq> []"] *}
-setup {* add_forward_prfstep_cond @{thm List.list.set_intros(1)} [with_term "set (?x21.0 # ?x22.0)"] *}
-setup {* add_forward_prfstep_cond @{thm List.list.set_intros(2)} [with_term "set (?x21.0 # ?x22.0)"] *}
-setup {* add_backward_prfstep @{thm List.list.set_intros(2)} *}
-setup {* add_rewrite_rule @{thm List.set_append} *}
-
-theorem in_set_conv_nth' [resolve]: "x \<in> set xs \<Longrightarrow> \<exists>i<length xs. x = xs ! i"
-  by (metis in_set_conv_nth)
+lemma length_Cons [rewrite]: "length (a # b) = length b + 1" by simp
+setup {* add_rewrite_rule @{thm length_tl} *}
+setup {* add_rewrite_rule @{thm List.length_append} *}
 
 section {* Showing two lists are equal *}
 
 setup {* add_backward2_prfstep_cond @{thm nth_equalityI} [with_filt (order_filter "xs" "ys")] *}
 
-section {* maps *}
+section {* nth *}
 
-setup {* add_rewrite_rule @{thm map_of.simps(1)} *}
-theorem map_of2 [rewrite]:
-  "map_of (p # ps) x = (if x = fst p then Some (snd p) else map_of ps x)" by simp
+setup {* register_wellform_data ("xs ! i", ["i < length xs"]) *}
+setup {* add_rewrite_rule_back @{thm hd_conv_nth} *}
+setup {* add_rewrite_rule @{thm List.nth_Cons'} *}
+setup {* add_rewrite_rule @{thm List.nth_append} *}
+
+section {* Set of elements of a list *}
+
+setup {* add_rewrite_rule @{thm List.set_simps(1)} *}
+lemma set_simps2 [rewrite]: "set (x # xs) = {x} \<union> set xs" by simp
+setup {* add_rewrite_rule @{thm List.set_append} *}
+setup {* add_resolve_prfstep @{thm List.finite_set} *}
+
+setup {* add_resolve_prfstep (equiv_forward_th @{thm in_set_conv_nth}) *}
+
+section {* sorted *}
+
+setup {* add_property_const @{term sorted} *}
+setup {* fold add_resolve_prfstep [@{thm sorted.Nil}, @{thm sorted_single}] *}
+setup {* add_backward_prfstep (equiv_backward_th @{thm sorted_Cons}) *}
+
+lemma sorted_ConsD1 [forward]: "sorted (x # xs) \<Longrightarrow> sorted xs" using sorted_Cons by blast
+lemma sorted_ConsD2 [forward, backward2]: "sorted (x # xs) \<Longrightarrow> y \<in> set xs \<Longrightarrow> x \<le> y"
+  using sorted_Cons by blast  
+
+lemma sorted_appendI [backward]:
+  "sorted xs \<Longrightarrow> sorted ys \<Longrightarrow> \<forall>x\<in>set xs. \<forall>y\<in>set ys. x \<le> y \<Longrightarrow> sorted (xs @ ys)"
+  by (simp add: sorted_append)
+
+section {* distinct *}
+
+setup {* add_property_const @{term distinct} *}
+  
+lemma distinct_Nil [resolve]: "distinct []" by simp
+setup {* add_resolve_prfstep @{thm List.distinct_singleton} *}
+
+lemma distinct_ConsI [backward]: "distinct xs \<Longrightarrow> \<forall>y\<in>set xs. x \<noteq> y \<Longrightarrow> distinct (x # xs)" by auto
+
+lemma distinct_ConsD1 [forward]: "distinct (x # xs) \<Longrightarrow> distinct xs" by auto
+lemma distinct_ConsD2 [forward]: "distinct (x # xs) \<Longrightarrow> x \<notin> set xs" by auto
+
+section {* map function *}
+
 setup {* fold add_rewrite_rule @{thms List.list.map} *}
 setup {* add_rewrite_rule @{thm List.map_append} *}
+
+section {* Replicate *}
+
+setup {* add_rewrite_rule @{thm length_replicate} *}
+setup {* add_rewrite_rule @{thm List.nth_replicate} *}
+
+section {* butlast *}
+
+setup {* add_rewrite_rule @{thm length_butlast} *}
+setup {* add_rewrite_rule @{thm nth_butlast} *}
+
+section {* List update *}
+
+setup {* register_wellform_data ("xs[i := x]", ["i < length xs"]) *}
+setup {* add_forward_prfstep_cond @{thm List.length_list_update} [with_term "?xs[?i := ?x]"] *}
+setup {* add_rewrite_rule @{thm List.nth_list_update_eq} *}
+setup {* add_rewrite_rule @{thm List.nth_list_update_neq} *}
+setup {* add_rewrite_rule @{thm List.nth_list_update} *}
+
+section {* take *}
+
+setup {* register_wellform_data ("take n xs", ["n \<le> length xs"]) *}
+setup {* add_prfstep_check_req ("take n xs", "n \<le> length xs") *}
+
+lemma length_take: "n \<le> length xs \<Longrightarrow> length (take n xs) = n" by simp
+setup {* add_rewrite_rule_cond @{thm length_take} [with_term "take ?n ?xs"] *}
+
+lemma nth_take [rewrite]: "i < length (take n xs) \<Longrightarrow> take n xs ! i = xs ! i" by simp
+
+setup {* add_rewrite_rule @{thm List.take_0} *}
+
+section {* drop *}
+
+setup {* add_rewrite_rule_cond @{thm List.length_drop} [with_term "drop ?n ?xs"] *}
+
+lemma nth_drop [rewrite]: "i < length (drop n xs) \<Longrightarrow> drop n xs ! i = xs ! (n + i)" by simp
+
+setup {* add_rewrite_rule @{thm List.drop_0} *}
+setup {* add_rewrite_rule @{thm List.drop_all} *}
+
+section {* rev *}
+
+setup {* add_forward_prfstep_cond @{thm List.length_rev} [with_term "rev ?xs"] *}
+setup {* fold add_rewrite_rule @{thms List.rev.simps} *}
+setup {* add_rewrite_rule @{thm List.rev_append} *}
+
+section {* mset *}
+
+setup {* add_rewrite_rule @{thm mset.simps(1)} *}
+lemma mset_simps_2 [rewrite]: "mset (a # x) = mset x + {#a#}" by simp
+setup {* add_rewrite_rule @{thm mset_append} *}
+setup {* add_backward2_prfstep @{thm mset_swap} *}
+
+setup {* add_rewrite_rule @{thm mset_eq_setD} *}
+lemma mset_butlast [forward]: "p \<in># mset (butlast xs) \<Longrightarrow> p \<in># mset xs" by (simp add: in_set_butlastD)
+setup {* add_rewrite_rule_cond @{thm in_multiset_in_set} [with_term "set ?xs"] *}
+setup {* add_rewrite_rule_back_cond @{thm in_multiset_in_set} [with_term "mset ?xs"] *}
+setup {* add_backward_prfstep @{thm Multiset.nth_mem_mset} *}
+
+lemma in_mset_conv_nth [resolve]: "x \<in># mset xs \<Longrightarrow> \<exists>i<length xs. x = xs ! i"
+  by (metis in_multiset_in_set in_set_conv_nth)
 
 end
